$$\begin{gather} u^\mu \equiv \frac{dx^\mu}{d\tau} \\ u_\mu u^\mu =c^2 \\ (cd\tau, 0) \to (cdt,d\vec x) \\ ds^2 =c^2 d\tau^2 = c^2dt^2 - d\vec x^2 \\ \left(\frac{d\tau}{dt}\right)^2 = 1 - \frac{1}{c^2}\left(\frac{d\vec x}{dt}\right)^2 = 1 - \frac{v^2}{c^2} = 1 -\beta^2 = \frac{1}{\gamma^2}\\dt = \gamma d\tau \\ u^\mu = (\gamma c,\gamma\vec v)\end{gather}$$

Note: $\frac{d\vec x}{dt}$ is not a 4-vector ($\vec x,t$ both transform)

$$\begin{gather} \frac{d\vec x}{dt} = \frac{1}{\gamma} \frac{d\vec x}{d\tau}=\frac{1}{\gamma}\vec v\end{gather}$$