If the boost $\beta$ is along the $x^1$ axis of $\{x\}$:

For $\vec \beta$ 

$$\begin{gather} L = \begin{bmatrix} \gamma & -\vec\beta\gamma \\ -\vec \beta\gamma & \delta_{ij} + \frac{\gamma -1}{\beta^2}\beta_i\beta_j\end{bmatrix} \end{gather}$$
Where: 

$$\begin{gather} \vec \beta = \beta_1\hat x^1 +\beta_2 \hat x^2 + \beta_3 \hat x^3 \end{gather}$$
explicitly: 

$$\begin{gather} x'^0 = \gamma(x^0-\beta \cdot \vec x) = \gamma(x^0-\beta x_\parallel) \\ \vec x = -\gamma \vec \beta x^0 + \vec x + \frac{\gamma-1}{\beta^2}(\vec \beta \cdot\vec x) \vec\beta \end{gather}$$

For the spatial part: 

$$\begin{gather} x_\parallel' = \gamma(x_\parallel - \beta x^0) \\ \vec x'_\perp = \vec x_\perp \end{gather}$$