Assuming a constructed Lagrangian is given.

1) Perform the [[Legendre Transform]] to convert $\mathcal L \to \mathcal H$: $$\begin{gather} \mathcal H(\{q,p\}) = \sum_jp_jv_j(\{q,p\}) - \mathcal L (\{q,v(\{q,p\})\})\end{gather}$$ and $p_j$ is defined as: $$\begin{gather} p_j = \frac{\partial \mathcal L}{\partial \dot q_j} \end{gather}$$ and $v_j$: $$\begin{gather} \dot q = v \end{gather}$$
2) Introduce [[Complex Canonical Variables]] $\{a_j, a^*_j*\}$: $$\begin{gather} a_j = \alpha q_j + i\beta p_j \\ a^*_j = \alpha^* q_j - i\beta^* p_j\end{gather}$$ We can also convert back by using the transform: $$\begin{gather} q_j = \lambda(\beta a_j^*+\beta^*a_j) \\ p_j = i\lambda(\alpha a_j^*-\alpha^*a_j)\end{gather}$$ Ideally, we want to use $\alpha$ and $\beta$ such that the value $\lambda$ defined by: $$\begin{gather} \lambda = \frac{1}{\alpha \beta^* + \alpha^*\beta} \end{gather}$$ is 1. 
3) Write out the Hamiltonian ([[Hamiltonian Function and Hamilton's Equations]]) with the new complex canonical variables. 
4) Find the components of the $A$ and $B$ matrices by using the formulas: $$\begin{gather} H = \sum_{ij}\left(A_{ij}a^*_ia_j + \frac{1}{2}B_{ij}a_ia_j +\frac{1}{2}B^*_{ij}a^*_ia^*_j\right) \\ A_{ij} = \frac{\partial^2  H}{\partial a_i\partial a_j^*}, \;\;\;\; B_{ij} = \frac{\partial^2 H}{\partial a_i\partial a_j} \\ A_{ij} = A_{ji}^*, \;\;\;\;\; B_ij = B_{ji}\end{gather}$$
5) Now we want to diagonalize the Hamiltonian so it takes the form: $$\begin{gather} \mathcal H = \sum_s \omega_sb_sb_s^* \end{gather}$$ Where $b_s$ is defined by:  $$\begin{gather} b_s = \sum_j(u_{sj}a_j + v_{sj}a^*_j) \end{gather}$$ 
6) Using the [[Poisson Brackets]] relation we write: $$\begin{gather} i\{H,b_s\} = \omega_sb_s \end{gather}$$ Which comes from the diagonalized Hamiltonian from step 5, and the definition: $$\begin{gather}i\dot b_s = i\{H,b_s\} = \sum_j\left[\frac{\partial b_s}{\partial a_j}\frac{\partial H}{\partial a^*_j}-\frac{\partial b_s}{\partial a_j^*}\frac{\partial H}{\partial a_j}\right] = \frac{\partial H}{\partial b^*_s} \end{gather}$$
7) Complete the above Poisson Bracket operation
8) Establish a system of equations from the Poisson Bracket: $$\begin{gather} \sum_i [A_{ij}u_{si} - B_{ji}v_{si}] = \omega_s u_{sj}, & \sum_i[B_{ji}^*u_{si}-A_{ji}v_{si}] = \omega_sv_{sj}\end{gather}$$
9) We can also write these in vector form: $$\begin{gather} A^*\ket{u_s} -B\ket{v_s}=\omega_s \ket{u_s} \\ B^*\ket{u_s} - A\ket{v_s} = \omega_s\ket{v_s} \end{gather}$$
10) Solve the system of equations for $u$ and $v$. 
11) Use $u$ and $v$ to solve for $\omega_s$