Defined as: $$\begin{align} \vec{I} = \frac{1}{\gamma}(\vec{v}\times \vec{L}) - \frac{\vec{r}}{r} \equiv \frac{m}{\gamma}[v^2\vec{r} - (\vec{r}\cdot \vec{v}) \vec{v}] - \frac{\vec{r}}{r} \end{align}$$

Which describes the shape and orientation of the orbit of one astronomical body around another, such as a binary star or a planet revolving around a star. For two bodies interacting by newtonian gravitty the LRL vector is a constant of motion.

[[How to Solve for Constants of Motion]]

Taking into account $\dot{\vec{L}}=0$, we get 
$$\begin{align} \dot{\vec{I}} = \frac{1}{\gamma}(\dot{v} \times \vec{L}) - \dot{r}/r + (\vec{r}/r^2)\dot{r} \\ \dot{r} = \frac{d}{dt}\sqrt{\vec{r}^2} = \frac{\vec{r}\cdot\dot{r}}{r} = \frac{\vec{r}\cdot\vec{v}}{r}\end{align}$$
From the equation of motion hwe have 
$$\begin{align} m\dot{\vec{v}} = -\frac{\partial}{\partial \vec{r}}(-\gamma/r) = \gamma\frac{\partial}{\partial \vec{r}} \frac{1}{\sqrt{\vec{r}^2}}  = - \gamma \frac{\vec{r}}{r^3} \rightarrow \dot{\vec{v}} = - \frac{\gamma}{m}\frac{\vec{r}}{r^3}  \end{align}$$

With $\vec{L} = m\vec{r} \times \vec{v}$\ we then find
$$\begin{align} \dot{I} = -\frac{1}{r^3}\vec{r} \times (\vec{r} \times \vec{v}) - \frac{\vec{v}}{r}+\frac{\vec{r}(\vec{r}\cdot\vec{v})}{r^3}\end{align}$$

Since
$$\begin{align} \vec{r} \times (\vec{r} \times\vec{v}) = \vec{r}(\vec{r}\cdot \vec{v}) - \vec{v}(\vec{r} \cdot \vec{r}) = \vec{r}(\vec{r} \cdot \vec{v}) - \vec{v}r^2\end{align}$$

we see that 
$$\begin{align} \dot{\vec{I}} = 0 \end{align}$$