Derive [[Snell's Law of Refraction]]:

![[problem 9.2 figure.png]]

$$\begin{align} \frac{ds}{dt} = \frac{c}{n} \\ dt = c^{-1}\int^B_A nds \\ = c^{-1}(n_1d_1 + n_2d_2)\end{align}$$

Where $d_1$ represents the distance $A\rightarrow P$ and $d_2$ represents the distance $P \rightarrow B$ 

Due to Fermat's theorem time is stationary, therefore $\frac{dt}{dx} = 0$.

$$\begin{align} \frac{dt}{dx} = c^{-1}\frac{d}{dx}\left(n_1\sqrt{(x_1 - x)^2 + (y_1 - 0)^2} + n_2\sqrt{(x - x_2)^2 + (0 - y_2)^2}\right) = 0 \\ = \frac{d}{dx}\left(n_1\sqrt{(x_1 - x)^2 + y_1^2} + n_2\sqrt{(x - x_2)^2 + y_2^2}\right) = 0\end{align}$$

Differentiate and equate to $\theta$ gives us:

$$\begin{align} n_1\sin\theta_1 = n_2\sin\theta_2\end{align}$$