1) Let $c$ be a constant. If $f(x) = c$, then $f'(x)=0$.
2) Let $n$ be a positive integer. If $f(x) = x^n$, then $f'(x) = nx^{n-1}$
3) Let $f(x)$ and $g(x)$ be differentiable and $k$ be a constant. Then each of the following equations holds

	[[Sum Rule]]. The derivative of the sum of a function $f$ and a function $g$ is the same as the sum of the derivative of $f$ and the derivative of $g$.
	$$\begin{align} \frac{d}{dx}(f(x)+g(x)) = \frac{d}{dx}(f(x)) + \frac{d}{dx}(g(x)) \end{align}$$
	that is $$\begin{align} j(x) = f(x) + g(x) \rightarrow j'(x) = f'(x) + g'(x)\end{align}$$
	
	[[Constant Multiple Rule]]. The ferivative of a constant $c$ multiplied by a function $f$ is the came as the constant multiplied by the derivative:
	$$\begin{align} \frac{d}{dx}(kf(x)) = k\frac{d}{dx}(f(x)) \end{align}$$
4) [[The Product Rule]] Let $f(x)$ and $g(x)$ be differentiable functions. Then $$\begin{align} \frac{d}{dx} (f(x)g(x)) = \frac{d}{dx}(f(x)) \cdot g(x) + \frac{d}{dx}(g(x))\cdot f(x)\end{align}$$
5) [[The Quotient Rule]] Let $f(x)$ and $g(x)$ be differentiable functions. Then $$\begin{align} \frac{d}{dx} \left(\frac{f(x)}{g(x)}\right) =\frac{\frac{d}{dx}(f(x))\cdot g(x) - \frac{d}{dx}(g(x))\cdot f(x)}{(g(x))^2} \end{align}$$
6) [[The Chain Rule]] $$\begin{align} (f \circ g)' (c) = f'(g(c)) \cdot g'(c) \end{align}$$
7) [[Implicit Differentiation]] 