Let the y-axis be vertical. We have 
$$\begin{align} \mathcal{L} = T - U \\ T = \frac{mv^2}{2}\\U = mgy \end{align}$$

where $m$ is the pendulum mass, $v^2 = \dot{x}^2 + \dot{y}^2$ is the square of the velocity, $g$ is the free-fall acceleration. Because of the constraint, the system is described by one generalized coordinate, the angle $\theta$ between the rode and the negative direction of the y-axis. We then notice that $v^2 = l^2\dot{\theta}^2$, $y=-l\cos\theta$, with $l$ is the length of the rod and thus 

$$\begin{align} \mathcal{L} = ml^2(\dot{\theta}^2/2+\omega^2\cos\theta), \;\; \omega^2 = g/l \end{align}$$

The Lagrange equation is: $$\begin{align} \ddot{\theta} =-\omega^2\sin\theta \end{align}$$