Plane pendulum driven by changing the length of the wire by some given law $l=l(t)$. The starting point is the same as in the case of fixed-length pendulum:

$$\begin{align} \mathcal{L} = T - U, \\ T = \frac{mv^2}{2},\\ U = mgy = - mgl\cos\theta\end{align}$$

$$\begin{align} v^2 = v_\perp + v_\parallel = l^2\dot{\theta}^2 + \dot{l}^2\end{align}$$

The Lagrangian then reads: $$\begin{align} \mathcal{L} = m \left[\frac{l^2(t)\dot{\theta}^2}{2}+gl(t)\cos\theta+\frac{\dot{l}^2(t)}{2}\right]\end{align}$$

The equation of motion can then be given by: $$\begin{align} \mathcal{L}\frac{d}{dt}[l^2(t)\dot{\theta}] = -gl(t)\sin\theta \end{align}$$