A repeated index once up and once down, is understood to be summed upon:
$$\lambda^1 \ket{v_1} + \lambda^2 \ket{v_2} +...+ \lambda^n \ket{v_n} = \sum^n_{\mu=1} \lambda^{\mu} \ket{v_{\mu}} = \lambda^{\mu} \ket{v_{\mu}}$$

Consider two bases , $\ket{e_\mu}$ and $\ket{e_\mu'}$

Then we can decompose each of the $\ket{e_\mu}$ s in components with respect to $\ket{e_\mu'}$: 
$$\ket{e_v}=\Lambda^\mu_\nu \ket{e_\mu'}$$ (Einstein Convention) 

this implies that, for a given vector $\ket{v}$ that has components $v^\mu$ on the basis $\ket{e_\mu}$ and components $v'^\mu$ on the basis $\ket{e_\mu'}$

$$\ket{v} = v'^\mu \ket{e_\mu'} = v^\nu \ket{e_\nu} = v^\nu \Lambda^\mu_\nu \ket{e_\mu'}$$ 

So that $(v')^\mu = \Lambda^\mu_\nu v^\nu$